Common/Finite.lean
@@ -1,0 +1,123 @@
+import Std.Data.HashSet
+
+class Finite (α : Type u) where
+  cardinality : Nat
+  enumerate : α → Fin cardinality
+  nth : Fin cardinality → α
+  nth_inverse_enumerate : nth ∘ enumerate = id
+  enumerate_inverse_nth : enumerate ∘ nth = id
+
+theorem Finite.surjective {α : Type u} [Finite α] {a b : Fin (Finite.cardinality α)} : nth a = nth b → a = b := λh₃ ↦
+  have h₁ := Finite.enumerate_inverse_nth (α := α)
+  have h₄ := congrArg enumerate h₃
+  have h₂ : ∀(x : Fin (Finite.cardinality α)), (enumerate ∘ nth) x = x := λ_↦h₁.substr rfl
+  have h₅ := Function.comp_apply.subst (h₂ a).symm
+  have h₆ := Function.comp_apply.subst (h₂ b).symm
+  h₅.substr $ h₆.substr h₄
+
+theorem Finite.injective {α : Type u} [Finite α] {a b : α} : enumerate a = enumerate b → a = b := λh₁↦
+  have h₂ := Finite.nth_inverse_enumerate (α := α)
+  have h₃ := congrArg nth h₁
+  have h₄ : ∀(x : α), (nth ∘ enumerate) x = x := λ_↦h₂.substr rfl
+  have h₅ := Function.comp_apply.subst (h₄ a).symm
+  have h₆ := Function.comp_apply.subst (h₄ b).symm
+  h₅.substr $ h₆.substr h₃
+
+def Finite.set (α : Type u) [Finite α] [BEq α] [Hashable α] : Std.HashSet α :=
+  match h: (Finite.cardinality α) with
+  | 0 => Std.HashSet.empty
+  | l+1 => set_worker Std.HashSet.empty ⟨l,h.substr (p := λx ↦ l < x) $ Nat.lt.base l⟩
+where set_worker (set : Std.HashSet α) (n : Fin (Finite.cardinality α)) : Std.HashSet α :=
+  let e := Finite.nth n
+  let set := set.insert e
+  match n with
+  | ⟨0,_⟩ => set
+  | ⟨m+1,h₁⟩ => set_worker set ⟨m, Nat.lt_of_succ_lt h₁⟩
+
+protected theorem Finite.set_worker_contains_self' (α : Type u) [Finite α] [BEq α] [Hashable α] [LawfulBEq α] (a : α) (oldSet : Std.HashSet α) (h₁ : oldSet.contains a) (n : Fin (Finite.cardinality α)) : (Finite.set.set_worker α oldSet n).contains a := by
+  cases n
+  case mk n h₂ =>
+    induction n generalizing oldSet
+    case zero => unfold set.set_worker; simp[h₁]
+    case succ m hm =>
+      unfold set.set_worker
+      exact hm (oldSet.insert (nth ⟨m + 1, h₂⟩)) (by simp[h₁]) (Nat.lt_of_succ_lt h₂)
+
+protected theorem Finite.set_worker_contains_self (α : Type u) [Finite α] [BEq α] [Hashable α] [LawfulBEq α] : ∀ (a : α) (set : Std.HashSet α), (Finite.set.set_worker α set (Finite.enumerate a)).contains a := by
+  intros a oldSet
+  unfold set.set_worker
+  rw[←Function.comp_apply (f := nth), Finite.nth_inverse_enumerate, id_def]
+  split
+  case h_1 => apply Std.HashSet.contains_insert_self
+  case h_2 =>
+    apply Finite.set_worker_contains_self'
+    exact Std.HashSet.contains_insert_self
+
+protected theorem Finite.set_worker_contains (α : Type u) [Finite α] [BEq α] [Hashable α] [LawfulBEq α] : ∀ (a : α) (set : Std.HashSet α) (o : Nat) (h₁ : Finite.enumerate a + o < Finite.cardinality α), (Finite.set.set_worker α set ⟨Finite.enumerate a + o, h₁⟩).contains a := by
+  intros a oldSet offset h₁
+  induction offset generalizing oldSet
+  case zero =>
+    exact Finite.set_worker_contains_self _ _ _
+  case succ p hi =>
+    unfold set.set_worker
+    simp
+    have : ↑(enumerate a) + p < cardinality α := Nat.lt_of_succ_lt $ (Nat.add_assoc (enumerate a) p 1).substr h₁
+    exact hi (oldSet.insert (nth ⟨↑(enumerate a) + (p + 1), h₁⟩)) this
+
+theorem Finite.set_contains (α : Type u) [Finite α] [BEq α] [Hashable α] [LawfulBEq α] : ∀ (a : α), (Finite.set α).contains a := λa ↦ by
+    unfold set
+    split
+    case h_1 h => exact (Fin.cast h $ Finite.enumerate a).elim0
+    case h_2 l h =>
+      let o := l - enumerate a
+      have h₁ : (Finite.enumerate a).val + o = l := by omega
+      have h₂ := Finite.set_worker_contains _ a Std.HashSet.empty o (by omega)
+      simp[h₁] at h₂
+      assumption
+
+protected theorem Finite.set_worker_size (α : Type u) [Finite α] [BEq α] [Hashable α] [LawfulBEq α]
+: ∀(set : Std.HashSet α) (n : Fin (Finite.cardinality α)) (_ : ∀(x : Fin (Finite.cardinality α)) (_ : x ≤ n),
+   ¬set.contains (Finite.nth x)), (Finite.set.set_worker α set n).size = set.size + n + 1
+:= by
+  intros set n h₂
+  simp at h₂
+  unfold Finite.set.set_worker
+  cases n
+  case mk n h₁ =>
+    split
+    case h_1 m isLt he =>
+      simp at he
+      simp[Std.HashSet.size_insert, Std.HashSet.mem_iff_contains, h₂, he]
+    case h_2 m isLt he =>
+      simp
+      have h₄ : m < n := have : n = m.succ := Fin.val_eq_of_eq he; this.substr (Nat.lt_succ_self m)
+      have h₅ : ∀ (x : Fin (cardinality α)), x ≤ ⟨m, Nat.lt_of_succ_lt isLt⟩ → ¬(set.insert (nth ⟨n, h₁⟩)).contains (nth x) = true := by
+        simp
+        intros x hx
+        constructor
+        case right => exact h₂ x (Nat.le_trans hx (Nat.le_of_lt h₄))
+        case left =>
+          have h₅ : x ≠ ⟨n, h₁⟩ := Fin.ne_of_val_ne $ Nat.ne_of_lt $ Nat.lt_of_le_of_lt hx h₄
+          have h₆ := Finite.surjective (α := α) (a := x) (b := ⟨n,h₁⟩)
+          exact Ne.symm (h₅ ∘ h₆)
+      have h₃ := Finite.set_worker_size α (set.insert (nth ⟨n, h₁⟩)) ⟨m, Nat.lt_of_succ_lt isLt⟩ (h₅)
+      rw[h₃]
+      simp at he
+      simp[he, Std.HashSet.size_insert]
+      split
+      case isFalse => rw[Nat.add_assoc, Nat.add_comm 1 m]
+      case isTrue hx =>
+        subst n
+        have h₂ := h₂ ⟨m+1,h₁⟩ (Fin.le_refl _)
+        have hx := Std.HashSet.mem_iff_contains.mp hx
+        exact absurd hx (Bool.eq_false_iff.mp h₂)
+termination_by _ n => n.val
+
+theorem Finite.set_size_eq_cardinality (α : Type u) [Finite α] [BEq α] [Hashable α] [LawfulBEq α] : (Finite.set α).size = Finite.cardinality α := by
+  unfold set
+  split
+  case h_1 h => exact Std.HashSet.size_empty.substr h.symm
+  case h_2 l h =>
+    rewrite(occs := .pos [3])[h]
+    have := Finite.set_worker_size α Std.HashSet.empty ⟨l,h.substr $ Nat.lt_succ_self l⟩ (λx _↦Bool.eq_false_iff.mp (Std.HashSet.contains_empty (a:=Finite.nth x)))
+    simp only [this, Std.HashSet.size_empty, Nat.zero_add]
