Common/HashSet.lean
@@ -1,0 +1,9 @@
+import Std.Data.HashSet
+import Common.Finite
+
+open Std.HashSet
+namespace Std.HashSet
+
+theorem finite_size {α : Type u} [Finite α] [BEq α] [LawfulBEq α] [Hashable α] (set : Std.HashSet α) : set.size ≤ Finite.cardinality α := by
+
+  sorry
